fixed field notation issue

test/Example.lean
@@ -1,34 +1,42 @@
-import LeanToolkit.TAlgebra
+import LeanToolkit
 
+--
+-- Boolean
+--
 namespace Boolean
 
 inductive T where
 | Bool
 
 inductive Term where
-| True
-| False
+| True | False
 | If (c t₁ t₂: Term)
 
+def countNodes: Term → Nat
+| .True => 1
+| .False => 1
+| .If c t₁ t₂ => 1 + countNodes c + countNodes t₁ + countNodes t₂
+
 inductive Val: Term → Prop
-| TT: Val .True
-| FF: Val .False
+| T: Val .True | F: Val .False
 
 inductive TRel: Term → T → Prop
 | TT: TRel .True .Bool
 | FF: TRel .False .Bool
 | If: TRel c .Bool → TRel t₁ τ → TRel t₂ τ → TRel (.If c t₁ t₂) τ
 
-theorem UniqueType (t: Term): TRel t τ₁ → TRel t τ₂ → τ₁ = τ₂ :=
-by
-  intros h₁ h₂
-  induction h₁ with
-  | TT => cases h₂; simp
-  | FF => cases h₂; simp
-  | If h₃ h₄ h₅ ih₁ ih₂ ih₃ => cases h₂; apply ih₂; assumption;
+theorem countNodes_pos: ∀ (t:Term), countNodes t > 0 := by
+  intros t;
+  induction t with
+  | True => simp[countNodes]
+  | False => simp[countNodes]
+  | If c t₁ t₂ c_ih t₁_ih t₂_ih => simp[countNodes]; simp[Nat.add_assoc]; simp[Nat.add_comm 1 _]
 
 end Boolean
 
+--
+-- Nat
+--
 namespace Nat
 
 inductive T where
@@ -39,50 +47,159 @@ inductive Term where
 | Succ (t: Term)
 | Pred (t: Term)
 
+def countNodes: Term → Nat
+| .Zero => 1
+| .Succ t => 1 + countNodes t
+| .Pred t => 1 + countNodes t
+
 inductive Val: Term → Prop
 | Z: Val .Zero
-| S: Val v → Val (.Succ v)
+| S (v: Term): Val v → Val (.Succ v)
 
 inductive TRel: Term → T → Prop where
 | Z: TRel .Zero .N
 | S: TRel t .N → TRel (.Succ t) .N
 | P: TRel t .N → TRel (.Pred t) .N
 
-theorem UniqueType (t: Term): TRel t τ₁ → TRel t τ₂ → τ₁ = τ₂ :=
-by
-  intros h₁ h₂
-  induction h₁ with
-  | Z => cases h₂; simp
-  | S h₃ ih => apply ih; cases h₂; assumption
-  | P h₃ ih => apply ih; cases h₂; assumption
-
+/-
+theorem countNodes_pos: ∀ (t:Term), countNodes t > 0 := by
+  intros t;
+  induction t with
+  | Zero => simp[countNodes]
+  | Succ t' t_ih => simp[countNodes, Nat.add_comm]
+  | Pred t t_ih => simp[countNodes, Nat.add_comm]
+-/
 end Nat
 
-inductive T := Boolean.T + Nat.T
+--
+--  STLC
+--
+namespace STLC
+
+inductive T: Type
+| Fn (τ₁ τ₂: T)
+
+abbrev Var := String
+
+abbrev Context := Var → T
+def augment (Γ: Context) (x: Var) (τ: T): Context := λv ↦ if v=x then τ else Γ v
+
+inductive Term where
+| V   (x: Var)
+| Abs (x: Var) (τ: T) (b: Term)
+| App (t₁ t₂: Term)
+
+def countNodes: Term → Nat
+| .V _       => 2
+| .Abs _ _ b => 3 + countNodes b
+| .App t₁ t₂ => 1 + countNodes t₁ + countNodes t₂
+
+inductive Val: Term → Prop
+| A (x: Var) (τ: T) (b: Term): Val (.Abs x τ t)
+
+inductive TRel: Context → Term → T → Prop where
+| V (x: Var) (τ: T): Γ x = τ → TRel Γ (.V x) τ
+| Abs (x: Var) (b: Term) (τ₁ τ₂: T):
+    TRel (augment Γ x τ₁) b τ₂ → TRel Γ (.Abs x τ₁ b) (.Fn τ₁ τ₂)
+| App (t₁ t₂: Term) (τ₁ τ₂: T):
+    TRel Γ t₁ (.Fn τ₁ τ₂) → TRel Γ t₂ τ₁ → TRel Γ (.App t₁ t₂) τ₂
+
+theorem countNodes_pos: ∀ (t:Term), countNodes t > 0 := by
+  intros t;
+  induction t with
+  | V x => simp[countNodes]
+  | Abs x τ b b_ih => simp[countNodes]; rw[Nat.add_comm]; simp
+  | App t₁ t₂ t₁_ih t₂_ih => simp[countNodes, Nat.add_assoc, Nat.add_comm 1 _]; simp[←Nat.add_assoc]
+
+end STLC
+
+#print STLC.T
+inductive T := Boolean.T |+ Nat.T |+ STLC.T
 #print T
 
-inductive Term := Boolean.Term + Nat.Term
+inductive Term := Boolean.Term |+ Nat.Term |+ STLC.Term
 | isZero (t: Term)
 #print Term
 
-inductive Val := Boolean.Val + Nat.Val
-#print Val
+fn countNodes := Boolean.countNodes |+ Nat.countNodes |+ STLC.countNodes
+| isZero t => 1 + countNodes t
+#print countNodes
 
-inductive TRel: Term → T → Prop := Boolean.TRel + Nat.TRel
-| iz: TRel t T.N → TRel (.isZero t) T.Bool
+def countNodes : Term → Nat := λ x ↦
+  match x with
+  | Term.True => 1
+  | Term.False => 1
+  | If c t₁ t₂ => 1 + countNodes c + countNodes t₁ + countNodes t₂
+  | Term.Zero => 1
+  | t.Succ => 1 + countNodes t
+  | t.Pred => 1 + countNodes t
+  | Term.V x => 2
+  | Term.Abs x τ b => 3 + countNodes b
+  | t₁.App t₂ => 1 + countNodes t₁ + countNodes t₂
+  | isZero t => 1 + countNodes t
 
-#print TRel
-
-#print CoeDep
-instance: CoeDep Term Term.True Boolean.Term where
-  coe := Boolean.Term.True
+def countNodes : Term → Nat := λ x ↦
+  let b (x: Boolean.Term) :=
+    match x with
+    | Boolean.Term.True => 1
+    | Boolean.Term.False => 1
+    | Boolean.Term.If c t₁ t₂ => 1 + countNodes c + countNodes t₁ + countNodes t₂
+  match x with
+  | Term.True => b Boolean.Term.True
+  | Term.False => b Boolean.Term.False
+  | Term.If c t₁ t₂ => b (Boolean.Term.If c t₁ t₂)
+  | Term.Zero => 1
+  | Term.Succ t => 1 + countNodes t
+  | Term.Pred t => 1 + countNodes t
+  | Term.V x => 2
+  | Term.Abs x τ b => 3 + countNodes b
+  | Term.App t₁ t₂ => 1 + countNodes t₁ + countNodes t₂
+  | Term.isZero t => 1 + countNodes t
 
 /-
-theorem UniqueType (t: Term): TRel t τ₁ → TRel t τ₂ → τ₁ = τ₂ :=
-by
-  intros h₁ h₂
-  induction h₁ with
-  | TT => apply Boolean.UniqueType t
-  | FF => apply Boolean.UniqueType
+def Boolean.countNodes.inner := fun x: Boolean.Term =>
+  Boolean.Term.brecOn x fun x f =>
+    (match (motive := (x : Boolean.Term) → Boolean.Term.below x → ℕ) x with
+      | Boolean.Term.True => fun x => 1
+      | Boolean.Term.False => fun x => 1
+      | c.If t₁ t₂ => fun x => 1 + x.1.1 + x.2.1.1 + x.2.2.1)
+      f
+
+#print Acc.rec
+#print Boolean.Term.rec
+#print Boolean.Term.below
+#print Boolean.Term.brecOn
+#print Boolean.countNodes
+
+#print Boolean.countNodes
+
+#eval countNodes Term.Zero
+
+inductive Val := Boolean.Val |+ Nat.Val |+ STLC.Val
+#print Val
+#check STLC.augment
+def Context := STLC.Var → T
+
+instance: AR.Tools.Compose.Common.SubType STLC.Context Context where
+  coe f := λ x ↦ f x
+
+fn augment := STLC.augment
+#check STLC.augment
+#print STLC.augment
+#check augment
+#print augment
+
+inductive TRel: Context → Term → T → Prop := Boolean.TRel |+ Nat.TRel |+ STLC.TRel
+| iz: TRel Γ t T.N → TRel Γ (.isZero t) T.Bool
+#print hidden.TRel
+#print TRel
+#print STLC.Context
+#print CoeDep
+
+/-
+theorem countNodes_pos: ∀ (t:Term), countNodes t > 0 := by
+  intros t;
+  induction t with
+  |
 -/
---end BN
+-/
