Compose.lean
@@ -1,0 +1,7 @@
+--
+--  Compose.lean
+--
+--    inductive type composition
+--
+import LeanToolkit.TypeSum
+import LeanToolkit.FnSum
