LeanToolkit/Coe.lean
@@ -1,0 +1,96 @@
+import LeanToolkit.Common
+--import Mathlib.Data.List.Defs
+
+open Lean Elab Command Lean.Meta Lean.Elab.Term
+open Lean.Parser.Term
+open Lean.Parser.Command
+open Meta
+open Std
+
+-- returns two arrays: array of arg names, and a corresponding array of arg types
+partial def typeToArgs'(t?: Option Expr) (ctxt:Array Name): CommandElabM (Array Name × Array Expr) := do --(TSyntaxArray `ident × TSyntaxArray `term) := do
+  --logInfo m!"cntxt: {ctxt}"
+  match t? with
+  | some t =>
+      match t with
+      | .forallE n t b bi =>
+          if bi.isExplicit then
+            let n' ← if n.isAnonymous then mkFreshBinderName else pure n
+            let t' := fillinBVars t ctxt
+            --logInfo m!"abstraction: {t} {ctxt} {t'}"
+            let r ← typeToArgs' (some b) (ctxt.push n)
+            return (r.1.push n', r.2.push t')
+          else
+            typeToArgs' (some b) ctxt
+      | _ => return (#[], #[])
+  | none => return (#[], #[])
+
+def typeToArgs (t?: Option Expr): CommandElabM (Array Name × Array Expr) := do
+  let (a,b) ← typeToArgs' t? #[]
+  return (a.reverse, b.reverse)
+
+def genForT(t composite: Name) (ctype: Expr) (cs': List TracedConstructor): CommandElabM Unit := do
+  let cs := cs'.filter (λ c ↦ c.source.toConstantVal.name == t)
+
+  -- coercion function name
+  let coe := mkIdent `coe
+  let coeFnName := mkIdent (((`coe).append t).append composite)
+
+  -- pattern matching expressions
+  let mut pexprs := #[]
+  for c in cs do
+    --logInfo m!"constructor {c.name}: {c.type}"
+    -- constructor parameters
+    let (x,y) ← typeToArgs c.type
+    let argIds := x.map mkIdent
+    let argIds_ts' := Array.zip argIds y
+
+    let argTerms ← argIds_ts'.mapM
+      (λ (id, t') ↦ do
+          --logInfo m!"names: {t'} {t}"
+          if t'.constName == composite then `(($coeFnName $id)) else `($id))
+    let p ← `(matchAltExpr| | $(mkIdent (c.source.name.append c.name)) $argIds:term* =>
+                                    $(mkIdent <| composite.append c.name):ident $argTerms:term*)
+    pexprs := pexprs.push p
+
+  -- match expression
+  let param ← mkFreshBinderName
+  let m ← `(match $(mkIdent param):ident with $pexprs:matchAlt*)
+
+  -- instance name
+  let inst := mkIdent <| ((`SubType).append t).append composite
+
+  -- subtype instance command with ceorcion function
+  let (ids', ts') ← typeToArgs ctype
+  let ids := ids'.map mkIdent
+  let ts ← ts'.mapM (λ e ↦ liftTermElabM <| PrettyPrinter.delab e)
+  let bbs: TSyntaxArray `Lean.Parser.Term.bracketedBinder ←
+      (Array.zip ids ts).mapM (λ (n, t) ↦ `(bracketedBinder| ($n : $t)))
+
+  let coeFn ← `(def $coeFnName:ident $(mkIdent param):ident := $m)
+
+  let coeCmd ← `(instance $inst: ident $bbs:bracketedBinder* :
+                    $(mkIdent `SubType)
+                    ($(mkIdent t) $ids:ident*)
+                    ($(mkIdent composite) $ids:ident*)
+                    where $coe:ident := $coeFnName)
+
+  --logInfo m!"elaborating {coeFn}"
+  --logInfo m!"elaborating {coeCmd}"
+  -- elaborate instance command
+  elabCommand coeFn
+  elabCommand coeCmd
+
+def List.dedup [BEq α]: List α → List α
+| [] => []
+| x :: xs => if xs.contains x then dedup xs else x :: dedup xs
+
+def genCoeInst (composite: Name) (t: Expr) (cs: List TracedConstructor): CommandElabM Unit := do
+  let subtypes :=
+    List.filter (not ∘ Name.isPrefixOf `hidden) <|
+    List.dedup <| cs.map (ConstantVal.name ∘ InductiveVal.toConstantVal ∘ TracedConstructor.source)
+
+  -- type args
+
+  for s in subtypes do
+    genForT s composite t cs
