LeanToolkit/Common.lean
@@ -1,0 +1,125 @@
+--
+--  Common.lean
+--
+import Lean
+import Lean.Elab.Term
+import Lean.Elab.Deriving.Basic
+import Lean.Elab.Deriving.Util
+import Lean.Meta.Inductive
+import Lean.Meta.Transform
+
+open Lean
+open Elab
+open Command
+open Lean.Meta
+open Lean.Elab.Term
+open Lean.Parser.Term
+open Meta
+--open Std
+
+
+initialize envExt: EnvExtension (List (Name × Name)) ← registerEnvExtension (return [])
+
+structure TracedConstructor where
+  name:        Name
+  type:        Option Expr
+  source:      InductiveVal
+  extraParams: Nat
+
+class SubType (tSub tSuper: Type) extends Coe tSub tSuper
+
+instance PolySubType {α: Type → Type} {β γ: Type} [i: SubType β γ] [f: Functor α] : SubType (α β) (α γ) where
+  coe x := f.map i.coe x
+
+structure Binding where
+  name: Name
+  type: TSyntax `term
+  bi:   BinderInfo
+
+def constantInfo2Constructor (ci': Option ConstantInfo): TermElabM Constructor := do
+  match ci' with
+  | some ci =>
+      let cs := ci.name.components
+      let n := dite (cs ≠ []) (λ ne ↦ List.getLast cs ne) (λ _ ↦ Name.anonymous)
+      return (Constructor.mk n ci.type)
+  | _ => throwError "not a ConstantInfo object"
+
+def discardReturnType (e: Expr): Option Expr :=
+  match e with
+  | .forallE n t b bi =>
+        let o := discardReturnType b
+        match o with
+        | some e' => some (.forallE n t e' bi)
+        | none => t
+  | _ => none
+
+def fillinBVars (e: Expr) (bvars: Array Name) : Expr :=
+  e.replace λ e' ↦
+    match e' with
+    | .bvar n =>
+        if let some i := bvars[n]? then
+          some <| .const i []
+        else
+          none
+    | _ => none
+
+def genBinder (b: Binding): TermElabM (TSyntax `Lean.Parser.Term.bracketedBinder) := do
+  let t := b.type
+  if b.bi.isImplicit then
+    `(bracketedBinder| {$(mkIdent b.name) : $t})
+  else
+    `(bracketedBinder| ($(mkIdent b.name) : $t))
+
+def genBindings: List Binding → TermElabM (TSyntaxArray `Lean.Parser.Term.bracketedBinder)
+| []       => return #[]
+| b :: bs' => do
+    let h ← genBinder b
+    let t ← genBindings bs'
+    let all:TSyntaxArray `Lean.Parser.Term.bracketedBinder := TSyntaxArray.mk (h :: t.toList).toArray
+    return all
+
+def getExplicitParamTypes (e: Expr): List Expr :=
+  match e with
+  | .forallE _ t b bi =>
+        let o := getExplicitParamTypes b
+        if bi.isImplicit then o else t :: o
+  | _ => []
+
+def getInductiveVal(typ: Name): TermElabM InductiveVal := do
+  let env ← getEnv
+  let i := env.find? typ
+  match i with
+  | some j  => return j.inductiveVal!
+  | _       => throwError m!"{typ} is not an inductive value."
+
+def getTypeName: Expr → Name
+| .const c _        => c
+| .fvar v           => v.name
+| .app f _          => getTypeName f
+| .forallE _ _ b _  => getTypeName b
+| _                 => Name.anonymous
+
+def mkInstantiatedType (t: TSyntax `term): List Ident → TermElabM (TSyntax `term)
+| [] => return t
+| n :: ns' => do
+    let r ← `($t $n)
+    mkInstantiatedType r ns'
+
+def toParams
+  (e: Expr)
+  (bvars: Array Name)
+  (ignoreImplicit: Bool := true) :
+TermElabM (List Binding × Expr) := do
+  match e with
+  | .forallE n t b bi => do
+    let bvars' := if bi.isImplicit then bvars else bvars.insertIdx 0 n
+    let b' ← toParams b bvars'
+    let id := n --mkIdent n --(← mkFreshUserName `x)
+    let t' ← PrettyPrinter.delab (fillinBVars t bvars)
+    let r :=
+      if ignoreImplicit && bi.isImplicit then
+        b'
+      else
+        ⟨ ⟨id, t', bi⟩ :: b'.fst, fillinBVars b bvars'⟩
+    return r
+  | _ => return ⟨ [], fillinBVars e bvars⟩
