LeanToolkit/FnSum.lean
@@ -1,0 +1,173 @@
+--
+--  FnSum.lean
+--
+import LeanToolkit.Common
+import LeanToolkit.Subtype
+
+open Lean Elab Command Lean.Meta Lean.Elab.Term
+open Lean.Parser.Term
+open Lean.Parser.Command
+open Meta
+open Std
+
+namespace AR.Tools.Compose.FnSum
+
+set_option pp.fieldNotation false
+
+-- syntactic category for summing functions
+declare_syntax_cat functions
+
+abbrev altT := Lean.Parser.Term.matchAlt
+
+syntax (name := singleton) ident: functions
+syntax (name := funSum) functions " |+ " functions : functions
+--syntax (name := expAlts) functions : functions
+
+structure Fn where
+  name: Name
+  type: Expr
+  body: Expr
+  alts: Array Syntax
+
+private partial
+def getFnVals': TSyntax `functions → TermElabM (List Name)
+| `(functions| $i:ident) => return [i.getId]
+| `(functions| $l:functions |+ $r:functions) => do
+      let x ← getFnVals' l
+      let y ← getFnVals' r
+       return x ++ y
+| _ => return  []
+
+def adjustType (env: Environment) (t: Expr) (subs: List (Name × Name)): Expr :=
+  t.replace λ e ↦
+        match e.constName? with
+        | some n' => adjustSubTypeName env n' subs >>= (some ∘ mkConst)
+        | none => none
+
+#print ConstructorVal
+#print Constructor
+def extractAlts (n:Name) (e: Expr) (subs: List (Name × Name)): TermElabM (Array Syntax) := do
+  let env ← getEnv
+  let s := (e.find? λ e ↦
+    let e' := e.eq?
+    match e' with
+    | some (l, t, r) => t.isAppOf n
+    | _ => false)
+  let e' := if s.isSome then s.get! else e
+  let e' := e'.replace λ e ↦
+    let c := e.const?
+    match c with
+    | some (c', _) =>
+        let v? := env.find? c'
+        match v? with
+        | some (ConstantInfo.ctorInfo v) =>
+            some (mkConst (v.induct.append v.name) [])
+        | _ => none
+    | _ => none
+  let stx:Syntax ← PrettyPrinter.delab e'
+  logInfo m!"expression: {e'}"
+  logInfo m!"expression raw: {e'.dbgToString}"
+  logInfo m!"term: {stx}"
+  let m := stx.find? (λ s ↦ s.isOfKind `Lean.Parser.Term.matchAlts)
+
+  match m with
+  | some m' =>
+      let m' ← m'.replaceM λ stx ↦
+        let o := adjustSubTypeName env stx.getId subs
+        match o with
+        | some x => do
+            let r ← `($(mkIdent x))
+            return (some r)
+        | none => pure none
+      let x := m'.getNumArgs
+      let y := m'[0].getNumArgs
+      logInfo m!"arg count: {x} {y}"
+      return m'[0].getArgs
+  | none => return #[]
+
+def getFnVals (lhs: Name) (stx: TSyntax `functions) (subs: List (Name × Name)): CommandElabM (List Fn) := do
+  let fs' ← liftTermElabM <| getFnVals' stx
+  let fs := List.eraseDups fs'
+  logInfo m!"functions: {fs}"
+  --let env ← getEnv
+
+  fs.forM λ f ↦
+    addFnPair f lhs
+
+  fs.mapM λ f' ↦ do
+    let o ← liftTermElabM <| Lean.Meta.getUnfoldEqnFor? f'
+
+    --logInfo m!"looking for {o}"
+    let alts ←
+      match o with
+      | some n => do
+          liftTermElabM <| extractAlts f' ((← getConstInfo n).value!) subs
+      | _ => pure #[]
+
+    let t := (← getConstInfo f').type
+
+    return (Fn.mk f' t ((← getConstInfo f').value!) alts)
+
+def composeFns (subs: List (Name × Name)): List Fn → TermElabM Fn
+| [] => throwError "Empty list of functions."
+| x :: [] => do
+    let env ← getEnv
+    let t := adjustType env x.type subs
+    pure (Fn.mk x.name t x.body x.alts)
+| x :: xs => do
+    let env ← getEnv
+    let r ← composeFns subs xs
+    let t := adjustType env x.type subs
+    logInfo m!"comparing types {t} - {r.type}"
+    if (← isDefEq t r.type) then
+      logInfo m!"composing alts of dims {x.alts.size} and {r.alts.size}"
+      return (Fn.mk x.name t x.body (x.alts ++ r.alts))
+    else
+      throwError m!"Failed to sum up different types: {t} - {r.type}"
+#check matchAlts
+--
+--  elaborator for type sum syntax
+--
+elab "fn " d:ident sig':optDeclSig " := " fs':functions as:altT* : command => do
+  let lhs := d.getId
+
+  -- subtypes
+  let subs ← liftTermElabM <| findSubTypes
+  logInfo m!"subs: {subs}"
+  let (_, optSig) := expandOptDeclSig sig'
+  let expectedType ← optSig.bindM (λ s ↦ do pure <| some (← liftTermElabM <| elabType s))
+
+  let fs ← getFnVals lhs fs' subs.toList
+
+  logInfo m!"{fs.map Fn.name} - {fs.map Fn.type} - {fs.map Fn.body}"
+
+  let fn ← liftTermElabM <| composeFns subs.toList fs
+
+  logInfo m!"number of alts: {fn.alts.size}"
+
+  let (ps, r) ← liftTermElabM <| toParams fn.type #[]
+  let r' ← liftTermElabM <| PrettyPrinter.delab r
+
+  let mut p := `x
+
+  let sig ← liftTermElabM <| PrettyPrinter.delab fn.type
+    --match ps with
+    --| []      => throwError "empty parameter list"
+    --| x :: _  =>
+        --p := x.name
+    --    liftTermElabM <| genBindings ps
+
+  let body ←
+    if fn.alts.isEmpty then
+      liftTermElabM <| PrettyPrinter.delab fn.body
+    else
+      let xs := TSyntaxArray.mk (fn.alts ++ as.raw)
+      let v ← liftTermElabM <| mkFreshIdent sig
+      `(fun $v => match $v:ident with $xs:matchAlt*)
+
+  let cmd ← `(def $d : $sig := $body)
+
+  logInfo m!"elaborating {cmd}"
+  elabCommand cmd
+
+end AR.Tools.Compose.FnSum
