LeanToolkit/Subtype.lean
@@ -1,0 +1,57 @@
+--
+-- Subtype.lean
+--
+import LeanToolkit.Common
+
+open Lean Elab Command Lean.Meta Lean.Elab.Term Lean.Meta.SynthInstance
+open Lean.Parser.Term
+open Lean.Parser.Command
+open Meta
+open Std
+
+--
+-- find subtypes and their corresponding super-types in the current environment
+--
+def findSubTypes: TermElabM (Array (Name × Name)) := do
+  let env ← getEnv
+  --let st := env.find? `SubType
+  --let rs ← match st with
+  --          | some _ =>
+  --                try
+                    let stx ← `(SubType _ _)
+                    let t ← elabTerm stx none --false
+                    let rs ← getInstances t
+  --                catch _ => do
+  --                  return #[]
+  --          | none => return #[]
+
+  let relevantVals := Array.map (Expr.constName! ∘ Instance.val) rs
+  let relevantVals' := relevantVals.filterMap (λ v ↦  env.find? v)
+  let ts := relevantVals'.filterMap (λ v ↦
+    let w := (Expr.getAppArgs ∘ ConstantInfo.type) v
+    let p := Prod.mk (w[0]? >>= Expr.constName?) (w[1]? >>= Expr.constName?)
+    match p with
+    | ⟨ some x, some y ⟩ => some ⟨ x, y⟩
+    | _ => none
+    )
+  return ts
+
+def adjustFnName (env: Environment) (f: Name): Option Name := do
+  let envContents :=  EnvExtension.getState envExt env
+  let o := envContents.find? (λ (x,_) ↦ x.isPrefixOf f)
+  match o with
+  | some (x,y) => some (f.replacePrefix x y)
+  | none => none
+
+def addFnPair(x y: Name): CommandElabM Unit := do
+  let env ← getEnv
+  let envContents :=  EnvExtension.getState envExt env
+  let envContents := (x,y) :: envContents
+  modifyEnv (envExt.setState . envContents)
+
+def adjustSubTypeName (env: Environment)  (n: Name): List (Name × Name) → Option Name
+| [] => adjustFnName env n
+| ⟨tSub, tSuper⟩ :: xs =>
+    if tSub.isPrefixOf n then
+      (some (n.replacePrefix tSub tSuper)) else
+    adjustSubTypeName env n xs
