LeanToolkit/TypeSum.lean
@@ -1,0 +1,247 @@
+--
+-- TypeSum.lean
+--
+import LeanToolkit.Common
+import LeanToolkit.Subtype
+--import AR.Tools.Compose.CoeUp
+--import AR.Tools.Compose.CoeDown
+import LeanToolkit.Coe
+
+open Lean Elab Command Lean.Meta Lean.Elab.Term
+open Lean.Parser.Term
+open Lean.Parser.Command
+open Meta
+open Std
+
+-- syntactic category for summing types
+declare_syntax_cat types
+
+syntax (name := singleton) ident: types
+syntax (name := typeSum) types " |+ " types : types
+
+--
+-- create a new hidden inductive type with the explicit constructors
+-- then append the name of the created type to the list of types to
+-- be summed up
+--
+private def includeExplicitConstructors
+  (d: Ident)
+  (sig: TSyntax `Lean.Parser.Command.optDeclSig)
+  (cs : TSyntax `types)
+  (explicitCs: TSyntaxArray `Lean.Parser.Command.ctor): CommandElabM (TSyntax `types)
+:= do
+  let hiddenName := Name.append (Name.mkStr1 "hidden") d.getId
+  let ⟨_, s⟩  := expandOptDeclSig sig
+  -- logInfo m!"sig - {sig} - {s}"
+  let hiddenSig:TSyntax `Lean.Parser.Command.optDeclSig ←
+    if s.isSome then pure sig else `(optDeclSig| : Type)
+
+  let cmd ← `(inductive $d $hiddenSig where $explicitCs:ctor*)
+  -- logInfo m!"hidden command: {cmd}"
+
+  withNamespace (Name.mkStr1 "hidden") (elabCommand cmd)
+
+  `(types| $cs |+ $(mkIdent hiddenName):ident)
+
+--
+--  Given a type t, rename any occurrence of any of the sum constituents to the name of the sum type,
+--  and any occurrence of a name of a subtype to the name of its corresponding super-type.
+--
+private def adjustType
+  (t: Expr)
+  (lhs: Name)
+  (types: List InductiveVal)
+  (subs: List (Name × Name))
+: TermElabM Expr := do
+  let env ← getEnv
+  return Expr.replace
+    (λ e ↦
+        match e.constName? with
+        | some n' =>
+            if (types.map (ConstantVal.name ∘ InductiveVal.toConstantVal)).elem n' then
+              some (mkConst lhs)
+            else
+              match types.find? (λ n ↦ n.toConstantVal.name.isPrefixOf n') with
+              | some t => some (Lean.mkConst (n'.replacePrefix t.toConstantVal.name lhs))
+              | none => (adjustSubTypeName env n' subs) >>= (some ∘ mkConst)
+        | none =>
+            none
+    ) t
+
+--
+--  helper function for turning the constituent type names
+--  into a list of names
+--
+private partial
+def getTypeVals': TSyntax `types → TermElabM (List Name)
+| `(types| $i:ident) => do
+      if (← isInductive i.getId) then
+        return [i.getId]
+      else
+        throwError m!"{i.getId} is not inductive."
+| `(types| $l:types |+ $r:types) => do
+      let x ← getTypeVals' l
+      let y ← getTypeVals' r
+       return x ++ y
+| _ => return  []
+
+def getTypeVals(cs: TSyntax `types): TermElabM (List InductiveVal) := do
+  let ns ← getTypeVals' cs
+  let ns' := List.eraseDups ns
+  ns'.mapM getInductiveVal
+
+private def countExtraArgs (full part: Expr): TermElabM Nat := do
+  let (full', _) ← toParams full #[]
+  let (part', _) ← toParams part #[]
+  if full'.length >= part'.length then
+    return full'.length - part'.length
+  else
+    throwError m!"types {full} and {part} are incompatible."
+
+private def getTypeDeltas
+  (expectedType: Expr)
+  (types: List InductiveVal)
+  (lhs: Name)
+  (subs: List (Name × Name))
+: TermElabM (List Nat) := do
+  let ts ← types.mapM (λ x ↦ adjustType x.type lhs types subs)
+  let r  ← ts.mapM (λ x ↦ countExtraArgs expectedType x)
+  return r
+
+private def checkTypeCompat
+  (types: List InductiveVal)
+  (lhs: Name)
+  (subs: List (Name × Name))
+: TermElabM Expr := do
+  match types with
+  | [] => throwError m!"empty list of types"
+  | t :: ts =>
+      let t ← adjustType t.type lhs types subs
+      if ts.isEmpty then return t
+      else
+        let e ← checkTypeCompat ts lhs subs
+        let c ←
+          if ←((isDefEq t e))
+          then return e
+          else throwError m!"{t} and {e} are different types."
+
+def concatConstructors
+  (css: List (List TracedConstructor))
+: TermElabM (List TracedConstructor) := do
+  match css with
+  | [] => return []
+  | cs :: css' =>
+      let mut result: List TracedConstructor := cs
+      let c₂ ← concatConstructors css'
+      for c in c₂ do
+        if let some c' := result.find? (λ c'' ↦ c.name == c''.name) then
+          if c.type != c'.type then
+            throwError "constructors of same name and mismatching types"
+        else result := result.append [c]
+      return result
+
+private def getCtors (typ : InductiveVal × Nat): TermElabM (List TracedConstructor) := do
+  let env ← getEnv
+  let ci := List.map (λ c ↦ (env.find? c)) typ.1.ctors
+  let cs ← List.mapM constantInfo2Constructor ci
+  return List.map (λ c ↦ ⟨c.name, some c.type, typ.1, typ.2⟩) cs
+
+--
+--  implementation of the type sum elaborator
+--
+private def typeSumImp
+  (ts: List InductiveVal)
+  (expectedType?: Option Expr)
+  (lhs:Name)
+  (subs: List (Name × Name)):
+TermElabM (List (List TracedConstructor) × Expr × List Binding) := do
+  let mut e: Expr := .const (Name.anonymous) []
+  let mut deltas: List Nat := ts.map (λ _ ↦ 0)
+
+  match expectedType? with
+    | some t =>
+        deltas ← getTypeDeltas t ts lhs subs
+        e := t
+    | none =>
+      e ← checkTypeCompat ts lhs subs
+
+  --if deltas.isEmpty then throwError "Incompatible types"
+
+  let (bvars, _) ← toParams e #[]
+  --let ts := ts.map getTypeName
+  --let ts := ts.eraseDups
+  --let ts ← ts.mapM getInductiveVal
+  let css ← (List.zip ts deltas).mapM getCtors
+
+  return ⟨css, e, bvars⟩
+
+def adjustConstructorType (name: Name) (e: Expr) (extraArgs: Nat): Expr :=
+  if extraArgs = 0 then e else
+    let dontCare := .const (Name.mkStr1 "_") []
+    e.replace λ x ↦
+      match x with
+      | .app (.const n us) e' =>
+          if (n == name) then
+            some <| .app (.app (.const n us) dontCare)
+                         (adjustConstructorType name e' (extraArgs -1))
+          else
+            none
+      | _ => none
+
+--
+--  elaborator for type sum syntax
+--
+elab "inductive " d:ident sig':optDeclSig " := " cs':types explicitCs: ctor* : command => do
+  let mut cs := cs'
+  let lhs := d.getId
+
+  -- explicit constructors
+  if explicitCs.size > 0 then
+    cs ← includeExplicitConstructors d sig' cs explicitCs
+
+  -- subtypes
+  let subs ← liftTermElabM <| findSubTypes
+  let (_, optSig) := expandOptDeclSig sig'
+  let expectedType ← optSig.bindM (λ s ↦ do pure <| some (← liftTermElabM <| elabType s))
+
+  logInfo m!"expected type: {expectedType}"
+  let ts ← liftTermElabM <| getTypeVals cs
+  let ⟨css, e, _⟩ ← liftTermElabM <| typeSumImp ts expectedType lhs subs.toList
+  let cs' ← liftTermElabM <| concatConstructors css
+  let cObjs ← List.mapM (
+            λ n ↦ do
+              let r := n.type
+              --logInfo m!"discarding return: {n.type} - {r}"
+              let t' ←
+                (match r with
+                | some r' => do
+                              let x ← liftTermElabM <| adjustType r' lhs ts subs.toList
+                              return (some x)
+                | none => return none)
+              --logInfo m!"adjusted {n.type} to {t'}"
+              let t' := match t' with
+                        | some t => adjustConstructorType lhs t n.extraParams
+                        | none => t'
+              return TracedConstructor.mk n.name t' n.source n.extraParams) cs'
+
+  let cStx ← cObjs.mapM (λ c ↦ do
+        match c.type with
+        | some t' =>
+            let t ← liftTermElabM <| PrettyPrinter.delab t'
+            `(ctor| |$(mkIdent c.name):ident : $t:term)
+        | none => `(ctor| |$(mkIdent c.name):ident))
+
+  let e' ← liftTermElabM <| PrettyPrinter.delab e
+  let cmd ← `(inductive $(mkIdent lhs) : $e' $(cStx.toArray):ctor*)
+  logInfo m!"elaborating {cmd}"
+  elabCommand cmd
+
+  let s ← liftTermElabM <| getInductiveVal lhs
+  let propType ← liftTermElabM <| isPropFormerType s.type
+
+  if !propType then
+    genCoeInst lhs e cObjs
+    for t in ts do
+      let t ← liftTermElabM <| getInductiveVal t.name
+      --upCoe s t
+      --downCoe t s
