test/CaseStudy/Boolean.lean
@@ -1,0 +1,26 @@
+--
+-- Boolean
+--
+namespace Boolean
+
+inductive T where
+| Bool
+
+inductive Term where
+| True | False
+| If (c t₁ t₂: Term)
+
+def countNodes: Term → Nat
+| .True => 1
+| .False => 1
+| .If c t₁ t₂ => 1 + countNodes c + countNodes t₁ + countNodes t₂
+
+inductive Val: Term → Prop
+| T: Val .True | F: Val .False
+
+inductive TRel: Term → T → Prop
+| TT: TRel .True .Bool
+| FF: TRel .False .Bool
+| If: TRel c .Bool → TRel t₁ τ → TRel t₂ τ → TRel (.If c t₁ t₂) τ
+
+end Boolean
