test/CaseStudy/CaseStudy.lean
@@ -1,0 +1,42 @@
+import CaseStudy.Boolean
+import CaseStudy.Nat
+import CaseStudy.STLC
+import LeanToolkit
+
+set_option pp.fieldNotation false
+
+inductive T := Boolean.T |+ Nat.T |+ STLC.T
+#print T
+
+inductive Term := Boolean.Term |+ Nat.Term |+ STLC.Term
+| isZero (t: Term)
+#print Term
+#print hidden.Term
+
+fn countNodes := Boolean.countNodes |+ Nat.countNodes |+ STLC.countNodes
+| Term.isZero t => 1 + countNodes t
+#print countNodes
+
+inductive Val := Boolean.Val |+ Nat.Val |+ STLC.Val
+#print Val
+#check STLC.augment
+def Context := STLC.Var → T
+
+instance: SubType STLC.Context Context where
+  coe f := λ x ↦ f x
+
+fn augment := STLC.augment
+#check STLC.augment
+#print STLC.augment
+#check augment
+#print augment
+
+
+inductive TRel: Context → Term → T → Prop := Boolean.TRel |+ Nat.TRel |+ STLC.TRel
+| iz: TRel Γ t T.N → TRel Γ (Term.isZero t) T.Bool
+
+#print hidden.TRel
+#print TRel
+#print STLC.Context
+#print CoeDep
+#print hidden.Term
