test/CaseStudy/Nat.lean
@@ -1,0 +1,28 @@
+--
+-- Nat
+--
+namespace Nat
+
+inductive T where
+| N
+
+inductive Term where
+| Zero
+| Succ (t: Term)
+| Pred (t: Term)
+
+def countNodes: Term → Nat
+| .Zero => 1
+| .Succ t => 1 + countNodes t
+| .Pred t => 1 + countNodes t
+
+inductive Val: Term → Prop
+| Z: Val .Zero
+| S (v: Term): Val v → Val (.Succ v)
+
+inductive TRel: Term → T → Prop where
+| Z: TRel .Zero .N
+| S: TRel t .N → TRel (.Succ t) .N
+| P: TRel t .N → TRel (.Pred t) .N
+
+end Nat
