test/CaseStudy/STLC.lean
@@ -1,0 +1,34 @@
+--
+--  STLC
+--
+namespace STLC
+
+inductive T: Type
+| Fn (τ₁ τ₂: T)
+
+abbrev Var := String
+
+abbrev Context := Var → T
+def augment (Γ: Context) (x: Var) (τ: T): Context := λv ↦ if v=x then τ else Γ v
+
+inductive Term where
+| V   (x: Var)
+| Abs (x: Var) (τ: T) (b: Term)
+| App (t₁ t₂: Term)
+
+def countNodes: Term → Nat
+| .V _       => 2
+| .Abs _ _ b => 3 + countNodes b
+| .App t₁ t₂ => 1 + countNodes t₁ + countNodes t₂
+
+inductive Val: Term → Prop
+| A (x: Var) (τ: T) (b: Term): Val (.Abs x τ t)
+
+inductive TRel: Context → Term → T → Prop where
+| V (x: Var) (τ: T): Γ x = τ → TRel Γ (.V x) τ
+| Abs (x: Var) (b: Term) (τ₁ τ₂: T):
+    TRel (augment Γ x τ₁) b τ₂ → TRel Γ (.Abs x τ₁ b) (.Fn τ₁ τ₂)
+| App (t₁ t₂: Term) (τ₁ τ₂: T):
+    TRel Γ t₁ (.Fn τ₁ τ₂) → TRel Γ t₂ τ₁ → TRel Γ (.App t₁ t₂) τ₂
+
+end STLC
