test/K3.lean
@@ -1,0 +1,238 @@
+--
+-- Kleene K3 logic (logic of indeterminacy)
+--
+import AR.Tools.Compose
+import Lean
+
+--class TermOps (α: Type) where
+--  countNodes : α → Nat
+--  positiveSize : ∀ x: α, countNodes x > 0
+
+namespace Boolean
+
+inductive Term
+| T
+| F
+
+def countNodes (t: Term): Nat :=
+1 + match t with
+| .T => 1
+| .F => 1
+
+#check countNodes.eq_unfold
+
+theorem positiveSize: ∀x: Term, countNodes x > 0 :=
+by intros x; cases x <;> simp[countNodes]
+
+--instance (α: Σ T, TermOps T): TermOps (BTerm α) where
+--  countNodes := _countNodes α
+--  positiveSize := _positiveSize α
+
+end Boolean
+
+/-
+namespace Indet
+
+inductive Term
+| I
+
+def countNodes(t: Term): Nat :=
+1+ match t with
+| .I => 1
+
+theorem eq (t: Term): t = t := by rfl
+
+end Indet
+-/
+
+namespace Ops
+
+inductive Term
+| Neg (t: Term)
+| And (t₁ t₂: Term)
+| Or  (t₁ t₂: Term)
+| Imp (t₁ t₂: Term)
+
+def countNodes: Term → Nat
+| .Neg t      => 1 + countNodes t
+| .And t₁ t₂  => 1 + countNodes t₁ + countNodes t₂
+| .Or t₁ t₂   => 1 + countNodes t₁ + countNodes t₂
+| .Imp t₁ t₂  => 1 + countNodes t₁ + countNodes t₂
+
+theorem positiveSize: ∀x: Term, countNodes x > 0 :=
+by
+  intros x
+  cases x with
+  | Neg x   => simp[countNodes]; rw [Nat.one_add]; simp[Nat.zero_lt_succ]
+  | And x y => simp[countNodes]; rw [Nat.one_add, Nat.succ_add]; simp[Nat.zero_lt_succ]
+  | Or x y  => simp[countNodes]; rw [Nat.one_add, Nat.succ_add]; simp[Nat.zero_lt_succ]
+  | Imp x y => simp[countNodes]; rw [Nat.one_add, Nat.succ_add]; simp[Nat.zero_lt_succ]
+
+#print positiveSize
+--instance TTOps (α: Σ T, TermOps T): TermOps (Term α) where
+--  countNodes := _countNodes α
+--  positiveSize := _positiveSize α
+
+end Ops
+
+namespace BooleanLogic
+inductive Term := Boolean.Term |+ Ops.Term
+#print Term
+
+def countNodes(t: Term): Nat :=
+  match t with
+  | .T        => 1
+  | .F        => 1
+  | .Neg t    => 1 + (countNodes t)
+  | .And t₁ t₂  => 1 + countNodes t₁ + countNodes t₂
+  | .Or t₁ t₂   => 1 + countNodes t₁ + countNodes t₂
+  | .Imp t₁ t₂  => 1 + countNodes t₁ + (countNodes t₂)
+
+#print Ops.countNodes.eq_unfold
+--theorem positiveSize: ∀x: Term, countNodes x > 0 :=
+--by
+--  intros x; cases x <;> first | try apply Boolean.positiveSize | try apply Ops.positiveSize
+/-
+  intros x
+  induction x with
+  | T => simp[countNodes]
+  | F => simp[countNodes]
+  | Neg x   => simp[countNodes]; rw [Nat.one_add]; simp[Nat.zero_lt_succ]
+  | And x y => simp[countNodes]; rw [Nat.one_add, Nat.succ_add]; simp[Nat.zero_lt_succ]
+  | Or x y  => simp[countNodes]; rw [Nat.one_add, Nat.succ_add]; simp[Nat.zero_lt_succ]
+  | Imp x y ih₁ ih₂ => simp[countNodes]; apply Nat.lt_add_left; exact ih₂
+-/
+/-
+def countNodes: Term → Nat
+| Term.T => Boolean.countNodes Term.T
+| Term.F => Boolean.countNodes Term.F
+| Term.I => Indet.countNodes Term.I
+-/
+
+
+/-
+fn countNodes := Boolean.countNodes + Indet.countNodes + Ops.countNodes
+#print Term
+def countNodes (t: Term):  Nat :=
+  match t with
+  | .T => Boolean.countNodes .T
+  | .F => Boolean.countNodes .F
+  | .I => Indet.countNodes .I
+  | .Neg t => countNodes_Ops (.Neg t) --Term → Term
+where
+  countNodes_Ops (t: Term) :=
+  match t with
+  | .Neg t      => 1 + countNodes t
+  | .And t₁ t₂  => 1 + countNodes t₁ + countNodes t₂
+  | .Or t₁ t₂   => 1 + countNodes t₁ + countNodes t₂
+  | .Imp t₁ t₂  => 1 + countNodes t₁ + countNodes t₂
+  -/
+--Term.And : Term → Term → Term
+--Term.Or : Term → Term → Term
+--Term.Imp : Term → Term → Term
+
+--theorem eq (t: Term): t = t := Boolean.eq
+--by
+--  cases t with --first | apply Boolean.eq | apply Indet.eq | apply Ops.eq
+--  | T => apply Boolean.eq ↑.T
+--  | F => apply Boolean.eq
+--  | I => apply Indet.eq
+
+ --<;> first | apply Boolean.eq | apply Indet.eq | apply Ops.eq
+
+--inductive countNodes := Boolean.countNodes + Indet.countNodes
+--| .T => Boolean.countNodes .T
+--| .F => Boolean.countNodes .F
+--| .I => Indet.countNodes .I
+--| .Neg t => Ops.countNodes (.Neg t)
+
+
+
+--<;> Boolean.countNodes | Ops.countNodes
+
+--| .T => countNodes .T
+
+--BooleanLogic.Term.F : Term
+--BooleanLogic.Term.Neg : Term → Term
+--BooleanLogic.Term.And : Term → Term → Term
+--BooleanLogic.Term.Or : Term → Term → Term
+--BooleanLogic.Term.Imp : Term → Term → Term
+end BooleanLogic
+
+namespace K3Logic
+
+inductive Term := Boolean.Term |+ Indet.Term |+ Ops.Term
+#print Term
+end K3Logic
+
+namespace baseline
+inductive Term
+| T | F | I
+| Neg (t: Term)
+| And (t₁ t₂: Term)
+| Or  (t₁ t₂: Term)
+| Imp (t₁ t₂: Term)
+
+def countNodes: Term→ Nat
+| .T          => 1
+| .F          => 1
+| .I          => 1
+| .Neg t      => 1 + countNodes t
+| .And t₁ t₂  => 1 + countNodes t₁ + countNodes t₂
+| .Or t₁ t₂   => 1 + countNodes t₁ + countNodes t₂
+| .Imp t₁ t₂  => 1 + countNodes t₁ + countNodes t₂
+
+namespace Boolean
+
+inductive Term
+| T
+| F
+
+def countNodes: Term→ Nat
+| .T          => 1
+| .F          => 1
+
+end Boolean
+
+namespace Indet
+
+inductive Term
+| I
+
+def countNodes: Term → Nat
+| .I          => 1
+
+end Indet
+
+namespace Ops
+
+inductive Term
+| Neg (t: Term)
+| And (t₁ t₂: Term)
+| Or  (t₁ t₂: Term)
+| Imp (t₁ t₂: Term)
+
+def countNodes: Term→ Nat
+| .Neg t      => 1 + countNodes t
+| .And t₁ t₂  => 1 + countNodes t₁ + countNodes t₂
+| .Or t₁ t₂   => 1 + countNodes t₁ + countNodes t₂
+| .Imp t₁ t₂  => 1 + countNodes t₁ + countNodes t₂
+
+end Ops
+--
+-- def Lean.Meta.getConstUnfoldEqnFor? (declName : Name) :
+--MetaM (Option Name)
+
+--Returns the "const unfold" theorem (f.eq_unfold) for the given declaration. This is not extensible, and always builds on the unfold theorem (f.eq_def).
+
+#check countNodes.eq_unfold
+def x := Term.T
+#print x
+
+#check Term.brecOn
+#check Term.below
+#print Term.below
+#check Term.rec
+
+#print countNodes
+end baseline
