test/compose01.lean
@@ -1,0 +1,11 @@
+import AR.Tools.Compose
+
+inductive T1
+| C1
+| C2
+
+inductive T2 where
+| C3
+
+inductive sum := T1 |+ T2
+#print sum
